Fix indentation, closes #10

theories/PrettyPrinter.v
@@ -38,23 +38,14 @@ Fixpoint ppIndentation (n : nat) :=
 Definition string_of_list_aux {A} (f : A -> string) (sep : string) (l : list A) (indentation: nat): string :=
   let fix aux l :=
       match l return string with
-
       | nil => ""
       | cons a nil => ppIndentation indentation ++ f a
       | cons a l => ppIndentation indentation ++ f a ++ sep ++ aux l
       end
   in aux l.
 
-Definition string_of_list {A} (f : A -> string) (l : list A): string :=
-  string_of_list_aux f TkCR l 1.
-
-(* Instance PrettyKind : Pretty Kind := *)
-  (* fix pp k := *)
-    (* match k with *)
-    (* | Ced.KdStar => TkStar *)
-    (* | Ced.KdArrow k1 k2 => pp k1 ++ TkSpace ++ TkArrow ++ TkSpace ++ pp k2 *)
-    (* | Ced.KdPi k t => TkNotImpl *)
-    (* end. *)
+Definition string_of_list {A} (f : A -> string) (l : list A) (indentation: nat): string :=
+  string_of_list_aux f TkCR l indentation.
 
 Instance PrettyName : Pretty Name :=
   fun name =>
@@ -95,7 +86,7 @@ Instance PrettyParams : Pretty Params :=
 Definition ppDatatype (name : Var) (params: Params) (kind : Typ) (ctors : list Ctor) :=
   TkData ++ TkSpace ++ name ++ pretty params ++ TkSpace ++ TkColon ++ TkSpace
           ++ pretty kind ++ TkSpace ++ TkAssgn ++ TkCR
-          ++ string_of_list pretty ctors ++ TkDot.
+          ++ string_of_list pretty ctors 1 ++ TkDot.
 
 
 Instance PrettyDatatype : Pretty Cmd :=
@@ -106,6 +97,6 @@ Instance PrettyDatatype : Pretty Cmd :=
     end.
 
 Instance PrettyProgram : Pretty Program :=
-  fun p => string_of_list pretty p.
+  fun p => string_of_list pretty p 0.
 
 Local Close Scope string_scope.
